WIP re-state wp-rule for store

theories/rules/rules_Store.v
@@ -2,737 +2,745 @@ From iris.base_logic Require Export invariants gen_heap.
 From iris.program_logic Require Export weakestpre ectx_lifting.
 From iris.proofmode Require Import proofmode.
 From iris.algebra Require Import frac.
-From cap_machine Require Export rules_base.
+From cap_machine Require Export rules_base stdpp_extra.
 
 Section cap_lang_rules.
   Context `{memG Σ, regG Σ}.
   Context `{MachineParameters}.
   Implicit Types P Q : iProp Σ.
   Implicit Types σ : ExecConf.
-  Implicit Types c : cap_lang.expr. 
+  Implicit Types c : cap_lang.expr.
   Implicit Types a b : Addr.
   Implicit Types r : RegName.
-  Implicit Types v : cap_lang.val. 
-  Implicit Types w : Word.
-  Implicit Types reg : gmap RegName Word.
-  Implicit Types ms : gmap Addr Word.
+  Implicit Types v : Version.
+  Implicit Types lw: LWord.
+  Implicit Types reg : Reg.
+  Implicit Types lregs : LReg.
+  Implicit Types mem : Mem.
+  Implicit Types lmem : LMem.
 
-  Definition reg_allows_store (regs : Reg) (r : RegName) p b e a :=
-    regs !! r = Some (WCap p b e a) ∧
+  Definition reg_allows_store (lregs : LReg) (r : RegName) p b e a v :=
+    lregs !! r = Some (LCap p b e a v) ∧
     writeAllowed p = true ∧ withinBounds b e a = true.
 
-  Inductive Store_failure_store (regs: Reg) (r1 : RegName)(r2 : Z + RegName) (mem : gmap Addr Word):=
-  | Store_fail_const w:
-      regs !! r1 = Some w ->
-      is_cap w = false →
-      Store_failure_store regs r1 r2 mem
-  | Store_fail_bounds p b e a:
-      regs !! r1 = Some(WCap p b e a) ->
+  Inductive Store_failure_store (lregs: LReg) (r1 : RegName)(r2 : Z + RegName) (lmem : LMem):=
+  | Store_fail_const lw:
+      lregs !! r1 = Some lw ->
+      is_log_cap lw = false →
+      Store_failure_store lregs r1 r2 lmem
+  | Store_fail_bounds p b e a v:
+      lregs !! r1 = Some(LCap p b e a v) ->
       (writeAllowed p = false ∨ withinBounds b e a = false) →
-      Store_failure_store regs r1 r2 mem
+      Store_failure_store lregs r1 r2 lmem
   | Store_fail_invalid_PC:
-      incrementPC (regs) = None ->
-      Store_failure_store regs r1 r2 mem
-  .
-
-  Inductive Store_failure_incr (regs: Reg) (r1 : RegName)(r2 : Z + RegName) (mem : gmap Addr Word):=
+      incrementLPC (lregs) = None ->
+      Store_failure_store lregs r1 r2 lmem
   .
 
   Inductive Store_spec
-    (regs: Reg) (r1 : RegName) (r2 : Z + RegName)
-    (regs': Reg) (mem mem' : gmap Addr Word) : cap_lang.val → Prop
-  :=
-  | Store_spec_success p b e a storev oldv :
-      word_of_argument regs r2 = Some storev ->
-      reg_allows_store regs r1 p b e a  →
-      mem !! a = Some oldv →
-      mem' = (<[a := storev]> mem) →
-      incrementPC(regs) = Some regs' ->
-      Store_spec regs r1 r2 regs' mem mem' NextIV
+    (lregs: LReg) (r1 : RegName) (r2 : Z + RegName)
+    (lregs': LReg) (lmem lmem' : LMem) : cap_lang.val → Prop
+    :=
+  | Store_spec_success p b e a v storev oldv :
+    lword_of_argument lregs r2 = Some storev ->
+    reg_allows_store lregs r1 p b e a v →
+    lmem !! (a, v) = Some oldv →
+    lmem' = (<[(a, v) := storev]> lmem) →
+    incrementLPC(lregs) = Some lregs' ->
+    Store_spec lregs r1 r2 lregs' lmem lmem' NextIV
   | Store_spec_failure_store :
-      mem' = mem →
-      Store_failure_store regs r1 r2 mem ->
-      Store_spec regs r1 r2 regs' mem mem' FailedV.
+    lmem' = lmem →
+    Store_failure_store lregs r1 r2 lmem ->
+    Store_spec lregs r1 r2 lregs' lmem lmem' FailedV.
 
-  Definition allow_store_map_or_true (r1 : RegName) (regs : Reg) (mem : gmap Addr Word):=
-    ∃ p b e a,
-      read_reg_inr regs r1 p b e a ∧ 
-      if decide (reg_allows_store regs r1 p b e a) then
-        ∃ w, mem !! a = Some w
+  Definition allow_store_map_or_true (r1 : RegName) (lregs : LReg) (lmem : LMem):=
+    ∃ p b e a v,
+      read_reg_inr lregs r1 p b e a v ∧
+      if decide (reg_allows_store lregs r1 p b e a v) then
+        ∃ lw, lmem !! (a, v) = Some lw
       else True.
 
   Lemma allow_store_implies_storev:
-    ∀ (r1 : RegName)(r2 : Z + RegName) (mem0 : gmap Addr Word) (r : Reg) (p : Perm) (b e a : Addr) storev,
-      allow_store_map_or_true r1 r mem0
-      → r !! r1 = Some (WCap p b e a)
-      → word_of_argument r r2 = Some storev
+    ∀ (r1 : RegName) (r2 : Z + RegName) (lmem : LMem) (lregs : LReg)
+      (p : Perm) (b e a : Addr) v storev,
+      allow_store_map_or_true r1 lregs lmem
+      → lregs !! r1 = Some (LCap p b e a v)
+      → lword_of_argument lregs r2 = Some storev
       → writeAllowed p = true
       → withinBounds b e a = true
-      → ∃ (storev : Word),
-          mem0 !! a = Some storev.
+      → ∃ (storev : LWord),
+          lmem !! (a, v) = Some storev.
   Proof.
-    intros r1 r2 mem0 r p b e a storev HaStore Hr2v Hwoa Hwa Hwb.
+    intros r1 r2 lmem lregs p b e a v storev HaStore Hr2v Hwoa Hwa Hwb.
     unfold allow_store_map_or_true, read_reg_inr in HaStore.
-    destruct HaStore as (?&?&?&?& Hrinr & Hwo).
+    destruct HaStore as (?&?&?&?&?& Hrinr & Hwo).
     rewrite Hr2v in Hrinr. inversion Hrinr; subst.
     case_decide as Hra.
     - exact Hwo.
-    - contradiction Hra. done.
+    - contradiction Hra; done.
   Qed.
 
   Lemma mem_eq_implies_allow_store_map:
-    ∀ (regs : Reg)(mem : gmap Addr Word)(r1 : RegName)(w : Word) p b e a,
-      mem = <[a:=w]> ∅
-      → regs !! r1 = Some (WCap p b e a)
-      → allow_store_map_or_true r1 regs mem.
+    ∀ (lregs : LReg) (lmem : LMem)(r1 : RegName) (lw : LWord) p b e a v,
+      lmem = <[(a, v):= lw]> ∅
+      → lregs !! r1 = Some (LCap p b e a v)
+      → allow_store_map_or_true r1 lregs lmem.
   Proof.
-    intros regs mem r1 w p b e a Hmem Hrr2.
-    exists p,b,e,a; split.
+    intros lregs lmem r1 lw p b e a v Hmem Hrr2.
+    exists p,b,e,a,v; split.
     - unfold read_reg_inr. by rewrite Hrr2.
     - case_decide; last done.
-      exists w. simplify_map_eq. auto.
+      exists lw. simplify_map_eq. auto.
   Qed.
 
   Lemma mem_neq_implies_allow_store_map:
-    ∀ (regs : Reg)(mem : gmap Addr Word)(r1 : RegName)(pc_a : Addr)
-      (w w' : Word) p b e a,
-      a ≠ pc_a
-      → mem = <[pc_a:=w]> (<[a:=w']> ∅)
-      → regs !! r1 = Some (WCap p b e a)
-      → allow_store_map_or_true r1 regs mem.
+    ∀ (lregs : LReg) (lmem : LMem) (r1 : RegName) (pc_a : Addr) (pca_v : Version)
+      (lw lw' : LWord) p b e a v,
+      (a ≠ pc_a \/ v <> pca_v)
+      → lmem = <[(pc_a, pca_v):= lw]> (<[(a, v) := lw']> ∅)
+      → lregs !! r1 = Some (LCap p b e a v)
+      → allow_store_map_or_true r1 lregs lmem.
   Proof.
-    intros regs mem r1 pc_a w w' p b e a H4 Hrr2 Hreg1.
-    exists p,b,e,a; split.
+    intros lregs lmem r1 pc_a pca_v lw lw' p b e a v H4 Hrr2 Hreg1.
+    exists p,b,e,a,v; split.
     - unfold read_reg_inr. by rewrite Hreg1.
     - case_decide; last done.
-      exists w'. simplify_map_eq. auto.
+      exists lw'.
+      destruct H4; assert ((pc_a, pca_v) <> (a, v)) by congruence; simplify_map_eq; auto.
   Qed.
 
   Lemma mem_implies_allow_store_map:
-    ∀ (regs : Reg)(mem : gmap Addr Word)(r1 : RegName)(pc_a : Addr)
-      (w w' : Word) p b e a,
-      (if (a =? pc_a)%a
-       then mem = <[pc_a:=w]> ∅
-       else mem = <[pc_a:=w]> (<[a:=w']> ∅))
-      → regs !! r1 = Some (WCap p b e a)
-      → allow_store_map_or_true r1 regs mem.
+    ∀ (lregs : LReg) (lmem : LMem) (r1 : RegName) (pc_a : Addr) (pca_v : Version)
+      (lw lw' : LWord) p b e a v,
+      (if ((a,v) =? (pc_a, pca_v))%la
+       then lmem = <[(pc_a, pca_v):=lw]> ∅
+       else lmem = <[(pc_a, pca_v):=lw]> (<[(a, v):=lw']> ∅))
+      → lregs !! r1 = Some (LCap p b e a v)
+      → allow_store_map_or_true r1 lregs lmem.
   Proof.
-    intros regs mem r1 pc_a w w' p b e a H4 Hrr2.
-    destruct (a =? pc_a)%a eqn:Heq.
-      + apply Z.eqb_eq, finz_to_z_eq in Heq. subst a. eapply mem_eq_implies_allow_store_map; eauto.
-      + apply Z.eqb_neq in Heq.  eapply mem_neq_implies_allow_store_map; eauto. congruence.
+    intros lregs lmem r2 pc_a pca_v lw lw' p b e a v H4 Hrr2.
+    destruct ((a,v) =? (pc_a, pca_v))%la eqn:Heq; cbn in Heq.
+      + apply andb_true_iff in Heq. destruct Heq as [Heq1 Heq2].
+        apply Z.eqb_eq, finz_to_z_eq in Heq1. subst a.
+        apply Nat.eqb_eq in Heq2. subst v.
+        eapply mem_eq_implies_allow_store_map; eauto.
+      + apply andb_false_iff in Heq. destruct Heq as [Heq | Heq]
+      ; [ apply Z.eqb_neq in Heq |  apply Nat.eqb_neq in Heq ]
+      ; eapply (mem_neq_implies_allow_store_map _ _ _ pc_a pca_v _ _ _ _ _ a v) ; eauto.
+        left ; solve_addr.
   Qed.
 
-   Lemma wp_store Ep
-     pc_p pc_b pc_e pc_a
-     r1 (r2 : Z + RegName) w mem regs :
-   decodeInstrW w = Store r1 r2 →
-   isCorrectPC (WCap pc_p pc_b pc_e pc_a) →
-   regs !! PC = Some (WCap pc_p pc_b pc_e pc_a) →
-   regs_of (Store r1 r2) ⊆ dom regs →
-   mem !! pc_a = Some w →
-   allow_store_map_or_true r1 regs mem →
+  Lemma wp_store Ep
+    pc_p pc_b pc_e pc_a pc_v pca_v
+    r1 (r2 : Z + RegName) lw lmem lregs :
+    decodeInstrWL lw = Store r1 r2 →
+    isCorrectLPC (LCap pc_p pc_b pc_e pc_a pc_v) →
+    lregs !! PC = Some (LCap pc_p pc_b pc_e pc_a pc_v) →
+    regs_of (Store r1 r2) ⊆ dom lregs →
+    lmem !! (pc_a, pca_v) = Some lw →
+    allow_store_map_or_true r1 lregs lmem →
 
-   {{{ (▷ [∗ map] a↦w ∈ mem, a ↦ₐ w) ∗
-       ▷ [∗ map] k↦y ∈ regs, k ↦ᵣ y }}}
-     Instr Executable @ Ep
-   {{{ regs' mem' retv, RET retv;
-       ⌜ Store_spec regs r1 r2 regs' mem mem' retv⌝ ∗
-         ([∗ map] a↦w ∈ mem', a ↦ₐ w) ∗
-         [∗ map] k↦y ∈ regs', k ↦ᵣ y }}}.
-   Proof.
-     iIntros (Hinstr Hvpc HPC Dregs Hmem_pc HaStore φ) "(>Hmem & >Hmap) Hφ".
-     iApply wp_lift_atomic_head_step_no_fork; auto.
-     iIntros (σ1 ns l1 l2 nt) "[Hr Hm] /=". destruct σ1; simpl.
-     iDestruct (gen_heap_valid_inclSepM with "Hr Hmap") as %Hregs.
-
-     (* Derive necessary register values in r *)
-     pose proof (lookup_weaken _ _ _ _ HPC Hregs).
-     specialize (indom_regs_incl _ _ _ Dregs Hregs) as Hri. unfold regs_of in Hri.
-     feed destruct (Hri r1) as [r1v [Hr'1 Hr1]]. by set_solver+.
-     iDestruct (gen_mem_valid_inSepM mem mem0 with "Hm Hmem") as %Hma; eauto.
-
-     iModIntro.
-     iSplitR. by iPureIntro; apply normal_always_head_reducible.
-     iNext. iIntros (e2 σ2 efs Hpstep).
-     apply prim_step_exec_inv in Hpstep as (-> & -> & (c & -> & Hstep)).
-     iIntros "_".
-     iSplitR; auto. eapply step_exec_inv in Hstep; eauto.
-
-     rewrite /exec /= Hr1 /= in Hstep.
-
-     (* Now we start splitting on the different cases in the Store spec, and prove them one at a time *)
-
-     destruct (word_of_argument regs r2) as [ storev | ] eqn:HSV.
-     2: {
-       destruct r2 as [z | r2].
-       - cbn in HSV; inversion HSV.
-       - destruct (Hri r2) as [r0v [Hr0 _] ]. by set_solver+.
-         cbn in HSV. rewrite Hr0 in HSV. inversion HSV.
-     }
-     apply (word_of_arg_mono _ reg) in HSV as HSV'; auto. rewrite HSV' in Hstep. cbn in Hstep.
-
-     destruct (is_cap r1v) eqn:Hr1v.
-     2: { (* Failure: r1 is not a capability *)
-       assert (c = Failed ∧ σ2 = {| reg := reg ; mem := mem0 ; etable := etable ; enumcur := enumcur |}) as (-> & ->).
-       {
-         unfold is_cap in Hr1v.
-         destruct_word r1v; by simplify_pair_eq.
-       }
-       iFailWP "Hφ" Store_fail_const.
-     }
-     destruct r1v as [ | [p b e a | ] | ]; try inversion Hr1v. clear Hr1v.
-
-     destruct (writeAllowed p && withinBounds b e a) eqn:HWA.
-     2 : { (* Failure: r2 is either not within bounds or doesnt allow reading *)
-       inversion Hstep.
-       apply andb_false_iff in HWA.
-       iFailWP "Hφ" Store_fail_bounds.
-     }
-     apply andb_true_iff in HWA; destruct HWA as (Hwa & Hwb).
-
-     (* Prove that a is in the memory map now, otherwise we cannot continue *)
-     pose proof (allow_store_implies_storev r1 r2 mem regs p b e a storev) as (oldv & Hmema); auto.
-
-     (* Given this, prove that a is also present in the memory itself *)
-     iDestruct (gen_mem_valid_inSepM mem mem0 a oldv with "Hm Hmem" ) as %Hma' ; auto.
-
-      destruct (incrementPC regs ) as [ regs' |] eqn:Hregs'.
-      2: { (* Failure: the PC could not be incremented correctly *)
-        assert (incrementPC reg = None).
-        { eapply incrementPC_overflow_mono; first eapply Hregs'; eauto. }
-        rewrite incrementPC_fail_updatePC /= in Hstep; auto.
-        inversion Hstep.
-        cbn; iFrame; iApply "Hφ"; iFrame.
-        iPureIntro. eapply Store_spec_failure_store;eauto. by constructor.
-      }
-
-      iMod ((gen_mem_update_inSepM _ _ a) with "Hm Hmem") as "[Hm Hmem]"; eauto.
-
-     (* Success *)
-      rewrite /update_mem /= in Hstep.
-      eapply (incrementPC_success_updatePC _ (<[a:=storev]> mem0)) in Hregs'
-        as (p1 & g1 & b1 & e1 & a1 & a_pc1 & HPC'' & HuPC & ->).
-      eapply (updatePC_success_incl _ (<[a:=storev]> mem0)) in HuPC. 2: by eauto.
-      rewrite HuPC in Hstep; clear HuPC; inversion Hstep; clear Hstep; subst c σ2. cbn.
-
-      iFrame.
-      iMod ((gen_heap_update_inSepM _ _ PC) with "Hr Hmap") as "[Hr Hmap]"; eauto.
-      iFrame. iModIntro. iApply "Hφ". iFrame.
-      iPureIntro. eapply Store_spec_success; eauto.
-        * split; auto. exact Hr'1. all: auto.
-        * unfold incrementPC. rewrite a_pc1 HPC''. 
-      Unshelve. all: auto.
-   Qed.
-
-  Lemma wp_store_success_z_PC E pc_p pc_b pc_e pc_a pc_a' w z :
-     decodeInstrW w = Store PC (inl z) →
-     isCorrectPC (WCap pc_p pc_b pc_e pc_a) →
-     (pc_a + 1)%a = Some pc_a' →
-     writeAllowed pc_p = true →
-
-     {{{ ▷ PC ↦ᵣ WCap pc_p pc_b pc_e pc_a
-           ∗ ▷ pc_a ↦ₐ w }}}
-       Instr Executable @ E
-       {{{ RET NextIV;
-           PC ↦ᵣ WCap pc_p pc_b pc_e pc_a'
-              ∗ pc_a ↦ₐ (WInt z) }}}.
+    {{{ (▷ [∗ map] la↦lw ∈ lmem, la ↦ₐ lw) ∗
+          ▷ [∗ map] k↦y ∈ lregs, k ↦ᵣ y }}}
+      Instr Executable @ Ep
+      {{{ lregs' lmem' retv, RET retv;
+          ⌜ Store_spec lregs r1 r2 lregs' lmem lmem' retv⌝ ∗
+            ([∗ map] la↦lw ∈ lmem', la ↦ₐ lw) ∗
+            [∗ map] k↦y ∈ lregs', k ↦ᵣ y }}}.
   Proof.
-    iIntros (Hinstr Hvpc Hpca' Hwa φ)
-            "(>HPC & >Hi) Hφ".
-    iDestruct (map_of_regs_1 with "HPC") as "Hmap".
-    iDestruct (memMap_resource_1 with "Hi") as "Hmem".
+    iIntros (Hinstr Hvpc HPC Dregs Hmem_pc HaStore φ) "(>Hmem & >Hmap) Hφ".
+    (* iApply wp_lift_atomic_head_step_no_fork; auto. *)
+    (* iIntros (σ1 ns l1 l2 nt) "[Hr Hm] /=". destruct σ1; simpl. *)
+    (* iDestruct (gen_heap_valid_inclSepM with "Hr Hmap") as %Hregs. *)
 
-    iApply (wp_store with "[$Hmap $Hmem]"); eauto; simplify_map_eq; eauto.
-    { by rewrite !dom_insert; set_solver+. }
-    { eapply mem_eq_implies_allow_store_map; eauto. }
-    iNext. iIntros (regs' mem' retv) "(#Hspec & Hmem & Hmap)".
-    iDestruct "Hspec" as %Hspec.
+    (*  (* Derive necessary register values in r *) *)
+    (*  pose proof (lookup_weaken _ _ _ _ HPC Hregs). *)
+    (*  specialize (indom_regs_incl _ _ _ Dregs Hregs) as Hri. unfold regs_of in Hri. *)
+    (*  feed destruct (Hri r1) as [r1v [Hr'1 Hr1]]. by set_solver+. *)
+    (*  iDestruct (gen_mem_valid_inSepM mem mem0 with "Hm Hmem") as %Hma; eauto. *)
 
-    destruct Hspec. 
-     { (* Success *)
-       iApply "Hφ".
-       destruct H3 as [Hrr2 _]. simplify_map_eq.
-       rewrite memMap_resource_1.
-       incrementPC_inv.
-       simplify_map_eq.
-       rewrite !insert_insert.
-       iDestruct (regs_of_map_1 with "[$Hmap]") as "HPC"; eauto. iFrame. }
-     { (* Failure (contradiction) *)
-       destruct X; try incrementPC_inv; simplify_map_eq; eauto.
-       apply isCorrectPC_ra_wb in Hvpc. apply andb_prop_elim in Hvpc as [_ Hwb].
-       destruct o; last apply Is_true_false in H2. all:try congruence. done.
-     }
-   Qed.
+    (*  iModIntro. *)
+    (*  iSplitR. by iPureIntro; apply normal_always_head_reducible. *)
+    (*  iNext. iIntros (e2 σ2 efs Hpstep). *)
+    (*  apply prim_step_exec_inv in Hpstep as (-> & -> & (c & -> & Hstep)). *)
+    (*  iIntros "_". *)
+    (*  iSplitR; auto. eapply step_exec_inv in Hstep; eauto. *)
 
-   Lemma wp_store_success_reg_PC E src wsrc pc_p pc_b pc_e pc_a pc_a' w :
-     decodeInstrW w = Store PC (inr src) →
-     isCorrectPC (WCap pc_p pc_b pc_e pc_a) →
-     (pc_a + 1)%a = Some pc_a' →
-     writeAllowed pc_p = true →
+    (*  rewrite /exec /= Hr1 /= in Hstep. *)
 
-     {{{ ▷ PC ↦ᵣ WCap pc_p pc_b pc_e pc_a
-           ∗ ▷ pc_a ↦ₐ w
-           ∗ ▷ src ↦ᵣ wsrc }}}
-       Instr Executable @ E
-       {{{ RET NextIV;
-           PC ↦ᵣ WCap pc_p pc_b pc_e pc_a'
-              ∗ pc_a ↦ₐ wsrc
-              ∗ src ↦ᵣ wsrc }}}.
-   Proof.
-     iIntros (Hinstr Hvpc Hpca' Hwa φ)
-            "(>HPC & >Hi & >Hsrc) Hφ".
-     iDestruct (map_of_regs_2 with "HPC Hsrc") as "[Hmap %]".
-     iDestruct (memMap_resource_1 with "Hi") as "Hmem".
+    (*  (* Now we start splitting on the different cases in the Store spec, and prove them one at a time *) *)
 
-    iApply (wp_store with "[$Hmap $Hmem]"); eauto; simplify_map_eq; eauto.
-    { by rewrite !dom_insert; set_solver+. }
-    { eapply mem_eq_implies_allow_store_map; eauto.
-      all: by simplify_map_eq. }
-    iNext. iIntros (regs' mem' retv) "(#Hspec & Hmem & Hmap)".
-    iDestruct "Hspec" as %Hspec.
+    (*  destruct (word_of_argument regs r2) as [ storev | ] eqn:HSV. *)
+    (*  2: { *)
+    (*    destruct r2 as [z | r2]. *)
+    (*    - cbn in HSV; inversion HSV. *)
+    (*    - destruct (Hri r2) as [r0v [Hr0 _] ]. by set_solver+. *)
+    (*      cbn in HSV. rewrite Hr0 in HSV. inversion HSV. *)
+    (*  } *)
+    (*  apply (word_of_arg_mono _ reg) in HSV as HSV'; auto. rewrite HSV' in Hstep. cbn in Hstep. *)
 
-    destruct Hspec. 
-     { (* Success *)
-       iApply "Hφ".
-       destruct H4 as [Hrr2 _]. simplify_map_eq.
-       rewrite memMap_resource_1.
-       incrementPC_inv.
-       simplify_map_eq.
-       do 2 rewrite insert_insert.
-       iDestruct (regs_of_map_2 with "[$Hmap]") as "[HPC Hsrc]"; eauto. iFrame. }
-     { (* Failure (contradiction) *)
-       destruct X; try incrementPC_inv; simplify_map_eq; eauto.
-       apply isCorrectPC_ra_wb in Hvpc. apply andb_prop_elim in Hvpc as [_ Hwb].
-       destruct o; last apply Is_true_false in H3. congruence. done. congruence.
-     }
-    Qed.
+    (*  destruct (is_cap r1v) eqn:Hr1v. *)
+    (*  2: { (* Failure: r1 is not a capability *) *)
+    (*    assert (c = Failed ∧ σ2 = {| reg := reg ; mem := mem0 ; etable := etable ; enumcur := enumcur |}) as (-> & ->). *)
+    (*    { *)
+    (*      unfold is_cap in Hr1v. *)
+    (*      destruct_word r1v; by simplify_pair_eq. *)
+    (*    } *)
+    (*    iFailWP "Hφ" Store_fail_const. *)
+    (*  } *)
+    (*  destruct r1v as [ | [p b e a | ] | ]; try inversion Hr1v. clear Hr1v. *)
 
-   Lemma wp_store_success_reg_PC_same E pc_p pc_b pc_e pc_a pc_a' w w' :
-     decodeInstrW w = Store PC (inr PC) →
-     isCorrectPC (WCap pc_p pc_b pc_e pc_a) →
-     (pc_a + 1)%a = Some pc_a' →
-     writeAllowed pc_p = true →
+    (*  destruct (writeAllowed p && withinBounds b e a) eqn:HWA. *)
+    (*  2 : { (* Failure: r2 is either not within bounds or doesnt allow reading *) *)
+    (*    inversion Hstep. *)
+    (*    apply andb_false_iff in HWA. *)
+    (*    iFailWP "Hφ" Store_fail_bounds. *)
+    (*  } *)
+    (*  apply andb_true_iff in HWA; destruct HWA as (Hwa & Hwb). *)
 
-     {{{ ▷ PC ↦ᵣ WCap pc_p pc_b pc_e pc_a
-           ∗ ▷ pc_a ↦ₐ w }}}
-       Instr Executable @ E
-       {{{ RET NextIV;
-           PC ↦ᵣ WCap pc_p pc_b pc_e pc_a'
-              ∗ pc_a ↦ₐ WCap pc_p pc_b pc_e pc_a }}}.
-   Proof.
-     iIntros (Hinstr Hvpc Hpca' Hwa φ)
-            "(>HPC & >Hi) Hφ".
-     iDestruct (map_of_regs_1 with "HPC") as "Hmap".
-     iDestruct (memMap_resource_1 with "Hi") as "Hmem".
+    (*  (* Prove that a is in the memory map now, otherwise we cannot continue *) *)
+    (*  pose proof (allow_store_implies_storev r1 r2 mem regs p b e a storev) as (oldv & Hmema); auto. *)
 
-    iApply (wp_store with "[$Hmap $Hmem]"); eauto; simplify_map_eq; eauto.
-    { by rewrite !dom_insert; set_solver+. }
-    { eapply mem_eq_implies_allow_store_map; eauto.
-      all: by simplify_map_eq. }
-    iNext. iIntros (regs' mem' retv) "(#Hspec & Hmem & Hmap)".
-    iDestruct "Hspec" as %Hspec.
+    (*  (* Given this, prove that a is also present in the memory itself *) *)
+    (*  iDestruct (gen_mem_valid_inSepM mem mem0 a oldv with "Hm Hmem" ) as %Hma' ; auto. *)
 
-    destruct Hspec. 
-     { (* Success *)
-       iApply "Hφ".
-       destruct H3 as [Hrr2 _]. simplify_map_eq.
-       rewrite memMap_resource_1.
-       incrementPC_inv.
-       simplify_map_eq.
-       do 2 rewrite insert_insert.
-       iDestruct (regs_of_map_1 with "[$Hmap]") as "HPC"; eauto. iFrame. }
-      { (* Failure (contradiction) *)
-       destruct X; try incrementPC_inv; simplify_map_eq; eauto.
-       apply isCorrectPC_ra_wb in Hvpc. apply andb_prop_elim in Hvpc as [_ Hwb].
-       destruct o; last apply Is_true_false in H2. congruence. done. congruence.
-     }
-    Qed.
+    (*   destruct (incrementPC regs ) as [ regs' |] eqn:Hregs'. *)
+    (*   2: { (* Failure: the PC could not be incremented correctly *) *)
+    (*     assert (incrementPC reg = None). *)
+    (*     { eapply incrementPC_overflow_mono; first eapply Hregs'; eauto. } *)
+    (*     rewrite incrementPC_fail_updatePC /= in Hstep; auto. *)
+    (*     inversion Hstep. *)
+    (*     cbn; iFrame; iApply "Hφ"; iFrame. *)
+    (*     iPureIntro. eapply Store_spec_failure_store;eauto. by constructor. *)
+    (*   } *)
 
-   Lemma wp_store_success_same E pc_p pc_b pc_e pc_a pc_a' w dst z w'
-         p b e :
-     decodeInstrW w = Store dst (inl z) →
-     isCorrectPC (WCap pc_p pc_b pc_e pc_a) →
-     (pc_a + 1)%a = Some pc_a' →
-     writeAllowed p = true → withinBounds b e pc_a = true →
+    (*   iMod ((gen_mem_update_inSepM _ _ a) with "Hm Hmem") as "[Hm Hmem]"; eauto. *)
 
-     {{{ ▷ PC ↦ᵣ WCap pc_p pc_b pc_e pc_a
-           ∗ ▷ pc_a ↦ₐ w
-           ∗ ▷ dst ↦ᵣ WCap p b e pc_a }}}
-       Instr Executable @ E
-       {{{ RET NextIV;
-           PC ↦ᵣ WCap pc_p pc_b pc_e pc_a'
-              ∗ pc_a ↦ₐ (WInt z)
-              ∗ dst ↦ᵣ WCap p b e pc_a }}}.
-    Proof.
-     iIntros (Hinstr Hvpc Hpca' Hwa Hwb φ)
-            "(>HPC & >Hi & >Hdst) Hφ".
-     iDestruct (map_of_regs_2 with "HPC Hdst") as "[Hmap %]".
-     iDestruct (memMap_resource_1 with "Hi") as "Hmem".
+    (*  (* Success *) *)
+    (*   rewrite /update_mem /= in Hstep. *)
+    (*   eapply (incrementPC_success_updatePC _ (<[a:=storev]> mem0)) in Hregs' *)
+    (*     as (p1 & g1 & b1 & e1 & a1 & a_pc1 & HPC'' & HuPC & ->). *)
+    (*   eapply (updatePC_success_incl _ (<[a:=storev]> mem0)) in HuPC. 2: by eauto. *)
+    (*   rewrite HuPC in Hstep; clear HuPC; inversion Hstep; clear Hstep; subst c σ2. cbn. *)
 
-    iApply (wp_store _ pc_p with "[$Hmap $Hmem]"); eauto; simplify_map_eq; eauto.
-    { by rewrite !dom_insert; set_solver+. }
-    { eapply mem_eq_implies_allow_store_map; eauto.
-      all: by simplify_map_eq. }
-    iNext. iIntros (regs' mem' retv) "(#Hspec & Hmem & Hmap)".
-    iDestruct "Hspec" as %Hspec.
+    (*   iFrame. *)
+    (*   iMod ((gen_heap_update_inSepM _ _ PC) with "Hr Hmap") as "[Hr Hmap]"; eauto. *)
+    (*   iFrame. iModIntro. iApply "Hφ". iFrame. *)
+    (*   iPureIntro. eapply Store_spec_success; eauto. *)
+    (*     * split; auto. exact Hr'1. all: auto. *)
+    (*     * unfold incrementPC. rewrite a_pc1 HPC''.  *)
+    (*   Unshelve. all: auto. *)
+   (* Qed. *)
+  Admitted.
 
-    destruct Hspec. 
-     { (* Success *)
-       iApply "Hφ".
-       destruct H4 as [Hrr2 _]. simplify_map_eq.
-       rewrite memMap_resource_1.
-       incrementPC_inv.
-       simplify_map_eq.
-       do 2 rewrite insert_insert.
-       iDestruct (regs_of_map_2 with "[$Hmap]") as "[HPC Hsrc]"; eauto. iFrame. }
-     { (* Failure (contradiction) *)
-       destruct X; try incrementPC_inv; simplify_map_eq; eauto.
-       destruct o. all: congruence.
-     }
-     Qed.
+  (* Lemma wp_store_success_z_PC E pc_p pc_b pc_e pc_a pc_a' w z : *)
+  (*    decodeInstrW w = Store PC (inl z) → *)
+  (*    isCorrectPC (WCap pc_p pc_b pc_e pc_a) → *)
+  (*    (pc_a + 1)%a = Some pc_a' → *)
+  (*    writeAllowed pc_p = true → *)
 
-   Lemma wp_store_success_reg' E pc_p pc_b pc_e pc_a pc_a' w dst w'
-         p b e a :
-      decodeInstrW w = Store dst (inr PC) →
-     isCorrectPC (WCap pc_p pc_b pc_e pc_a) →
-     (pc_a + 1)%a = Some pc_a' →
-     writeAllowed p = true → withinBounds b e a = true →
+  (*    {{{ ▷ PC ↦ᵣ WCap pc_p pc_b pc_e pc_a *)
+  (*          ∗ ▷ pc_a ↦ₐ w }}} *)
+  (*      Instr Executable @ E *)
+  (*      {{{ RET NextIV; *)
+  (*          PC ↦ᵣ WCap pc_p pc_b pc_e pc_a' *)
+  (*             ∗ pc_a ↦ₐ (WInt z) }}}. *)
+  (* Proof. *)
+  (*   iIntros (Hinstr Hvpc Hpca' Hwa φ) *)
+  (*           "(>HPC & >Hi) Hφ". *)
+  (*   iDestruct (map_of_regs_1 with "HPC") as "Hmap". *)
+  (*   iDestruct (memMap_resource_1 with "Hi") as "Hmem". *)
 
-     {{{ ▷ PC ↦ᵣ WCap pc_p pc_b pc_e pc_a
-           ∗ ▷ pc_a ↦ₐ w
-           ∗ ▷ dst ↦ᵣ WCap p b e a
-           ∗ if (a =? pc_a)%a
-             then emp
-             else ▷ a ↦ₐ w' }}}
-       Instr Executable @ E
-       {{{ RET NextIV;
-           PC ↦ᵣ WCap pc_p pc_b pc_e pc_a'
-              ∗ pc_a ↦ₐ (if (a =? pc_a)%a
-                         then (WCap pc_p pc_b pc_e pc_a)
-                         else w)
-              ∗ dst ↦ᵣ WCap p b e a
-              ∗ if (a =? pc_a)%a
-                then emp
-                else a ↦ₐ (WCap pc_p pc_b pc_e pc_a) }}}.
-   Proof.
-     iIntros (Hinstr Hvpc Hpca' Hwa Hwb φ)
-            "(>HPC & >Hi & >Hdst & Ha) Hφ".
-     iDestruct (map_of_regs_2 with "HPC Hdst") as "[Hmap %]".
-     iDestruct (memMap_resource_2gen_clater _ _ _ _ (λ a w, a ↦ₐ w)%I  with "Hi Ha") as (mem) "[>Hmem %]".
+  (*   iApply (wp_store with "[$Hmap $Hmem]"); eauto; simplify_map_eq; eauto. *)
+  (*   { by rewrite !dom_insert; set_solver+. } *)
+  (*   { eapply mem_eq_implies_allow_store_map; eauto. } *)
+  (*   iNext. iIntros (regs' mem' retv) "(#Hspec & Hmem & Hmap)". *)
+  (*   iDestruct "Hspec" as %Hspec. *)
 
-    iApply (wp_store with "[$Hmap $Hmem]"); eauto; simplify_map_eq; eauto.
-    { by rewrite !dom_insert; set_solver+. }
-    { destruct (a =? pc_a)%a; by simplify_map_eq. }
-    { eapply mem_implies_allow_store_map; eauto. all: by simplify_map_eq. }
+  (*   destruct Hspec.  *)
+  (*    { (* Success *) *)
+  (*      iApply "Hφ". *)
+  (*      destruct H3 as [Hrr2 _]. simplify_map_eq. *)
+  (*      rewrite memMap_resource_1. *)
+  (*      incrementPC_inv. *)
+  (*      simplify_map_eq. *)
+  (*      rewrite !insert_insert. *)
+  (*      iDestruct (regs_of_map_1 with "[$Hmap]") as "HPC"; eauto. iFrame. } *)
+  (*    { (* Failure (contradiction) *) *)
+  (*      destruct X; try incrementPC_inv; simplify_map_eq; eauto. *)
+  (*      apply isCorrectPC_ra_wb in Hvpc. apply andb_prop_elim in Hvpc as [_ Hwb]. *)
+  (*      destruct o; last apply Is_true_false in H2. all:try congruence. done. *)
+  (*    } *)
+  (*  Qed. *)
 
-    iNext. iIntros (regs' mem' retv) "(#Hspec & Hmem & Hmap)".
-    iDestruct "Hspec" as %Hspec.
+  (*  Lemma wp_store_success_reg_PC E src wsrc pc_p pc_b pc_e pc_a pc_a' w : *)
+  (*    decodeInstrW w = Store PC (inr src) → *)
+  (*    isCorrectPC (WCap pc_p pc_b pc_e pc_a) → *)
+  (*    (pc_a + 1)%a = Some pc_a' → *)
+  (*    writeAllowed pc_p = true → *)
 
-    destruct Hspec. 
-     { (* Success *)
-       iApply "Hφ".
-       destruct H5 as [Hrr2 _]. simplify_map_eq.
-       destruct (a0 =? pc_a)%a eqn:Heq; subst mem.
-       -  apply Z.eqb_eq, finz_to_z_eq in Heq. subst a0.
-          rewrite insert_insert.
-          rewrite memMap_resource_1.
-          incrementPC_inv.
-          simplify_map_eq. rewrite insert_insert.
-          iDestruct (regs_of_map_2 with "[$Hmap]") as "[HPC Hsrc]"; eauto. iFrame.
+  (*    {{{ ▷ PC ↦ᵣ WCap pc_p pc_b pc_e pc_a *)
+  (*          ∗ ▷ pc_a ↦ₐ w *)
+  (*          ∗ ▷ src ↦ᵣ wsrc }}} *)
+  (*      Instr Executable @ E *)
+  (*      {{{ RET NextIV; *)
+  (*          PC ↦ᵣ WCap pc_p pc_b pc_e pc_a' *)
+  (*             ∗ pc_a ↦ₐ wsrc *)
+  (*             ∗ src ↦ᵣ wsrc }}}. *)
+  (*  Proof. *)
+  (*    iIntros (Hinstr Hvpc Hpca' Hwa φ) *)
+  (*           "(>HPC & >Hi & >Hsrc) Hφ". *)
+  (*    iDestruct (map_of_regs_2 with "HPC Hsrc") as "[Hmap %]". *)
+  (*    iDestruct (memMap_resource_1 with "Hi") as "Hmem". *)
 
-       - apply Z.eqb_neq in Heq.
-         rewrite insert_commute; last congruence. rewrite insert_insert.
-         iDestruct (memMap_resource_2ne with "Hmem") as "[Ha0 Hpc_a]"; first congruence.
-         incrementPC_inv.
-         rewrite lookup_insert_ne in H6; last congruence. simplify_map_eq. rewrite insert_insert.
-         iDestruct (regs_of_map_2 with "[$Hmap]") as "[HPC Hsrc]"; eauto. iFrame.
-     }
-     { (* Failure (contradiction) *)
-       destruct X; try incrementPC_inv; simplify_map_eq; eauto.
-       destruct o. all: try congruence.
-     }
-   Qed.
+  (*   iApply (wp_store with "[$Hmap $Hmem]"); eauto; simplify_map_eq; eauto. *)
+  (*   { by rewrite !dom_insert; set_solver+. } *)
+  (*   { eapply mem_eq_implies_allow_store_map; eauto. *)
+  (*     all: by simplify_map_eq. } *)
+  (*   iNext. iIntros (regs' mem' retv) "(#Hspec & Hmem & Hmap)". *)
+  (*   iDestruct "Hspec" as %Hspec. *)
 
-   Lemma wp_store_success_reg_frominstr_same E pc_p pc_b pc_e pc_a pc_a' w dst w'
-         p b e :
-      decodeInstrW w = Store dst (inr PC) →
-     isCorrectPC (WCap pc_p pc_b pc_e pc_a) →
-     (pc_a + 1)%a = Some pc_a' →
-     writeAllowed p = true →
-     withinBounds b e pc_a = true →
+  (*   destruct Hspec.  *)
+  (*    { (* Success *) *)
+  (*      iApply "Hφ". *)
+  (*      destruct H4 as [Hrr2 _]. simplify_map_eq. *)
+  (*      rewrite memMap_resource_1. *)
+  (*      incrementPC_inv. *)
+  (*      simplify_map_eq. *)
+  (*      do 2 rewrite insert_insert. *)
+  (*      iDestruct (regs_of_map_2 with "[$Hmap]") as "[HPC Hsrc]"; eauto. iFrame. } *)
+  (*    { (* Failure (contradiction) *) *)
+  (*      destruct X; try incrementPC_inv; simplify_map_eq; eauto. *)
+  (*      apply isCorrectPC_ra_wb in Hvpc. apply andb_prop_elim in Hvpc as [_ Hwb]. *)
+  (*      destruct o; last apply Is_true_false in H3. congruence. done. congruence. *)
+  (*    } *)
+  (*   Qed. *)
 
-     {{{ ▷ PC ↦ᵣ WCap pc_p pc_b pc_e pc_a
-           ∗ ▷ pc_a ↦ₐ w
-           ∗ ▷ dst ↦ᵣ WCap p b e pc_a }}}
-       Instr Executable @ E
-       {{{ RET NextIV;
-           PC ↦ᵣ WCap pc_p pc_b pc_e pc_a'
-              ∗ pc_a ↦ₐ WCap pc_p pc_b pc_e pc_a
-              ∗ dst ↦ᵣ WCap p b e pc_a }}}.
-   Proof.
-     intros. iIntros "(HPC & Hpc_a & Hdst) Hφ".
-     iApply (wp_store_success_reg' with "[$HPC $Hpc_a $Hdst]"); eauto.
-     { rewrite Z.eqb_refl. eauto. }
-     iNext. iIntros "(? & ? & ? & ?)". rewrite Z.eqb_refl.
-     iApply "Hφ". iFrame. Unshelve. eauto.
-   Qed.
+  (*  Lemma wp_store_success_reg_PC_same E pc_p pc_b pc_e pc_a pc_a' w w' : *)
+  (*    decodeInstrW w = Store PC (inr PC) → *)
+  (*    isCorrectPC (WCap pc_p pc_b pc_e pc_a) → *)
+  (*    (pc_a + 1)%a = Some pc_a' → *)
+  (*    writeAllowed pc_p = true → *)
 
-   Lemma wp_store_success_reg_frominstr E pc_p pc_b pc_e pc_a pc_a' w dst w'
-         p b e a :
-      decodeInstrW w = Store dst (inr PC) →
-     isCorrectPC (WCap pc_p pc_b pc_e pc_a) →
-     (pc_a + 1)%a = Some pc_a' →
-     writeAllowed p = true →
-     withinBounds b e a = true →
+  (*    {{{ ▷ PC ↦ᵣ WCap pc_p pc_b pc_e pc_a *)
+  (*          ∗ ▷ pc_a ↦ₐ w }}} *)
+  (*      Instr Executable @ E *)
+  (*      {{{ RET NextIV; *)
+  (*          PC ↦ᵣ WCap pc_p pc_b pc_e pc_a' *)
+  (*             ∗ pc_a ↦ₐ WCap pc_p pc_b pc_e pc_a }}}. *)
+  (*  Proof. *)
+  (*    iIntros (Hinstr Hvpc Hpca' Hwa φ) *)
+  (*           "(>HPC & >Hi) Hφ". *)
+  (*    iDestruct (map_of_regs_1 with "HPC") as "Hmap". *)
+  (*    iDestruct (memMap_resource_1 with "Hi") as "Hmem". *)
 
-     {{{ ▷ PC ↦ᵣ WCap pc_p pc_b pc_e pc_a
-           ∗ ▷ pc_a ↦ₐ w
-           ∗ ▷ dst ↦ᵣ WCap p b e a
-           ∗ ▷ a ↦ₐ w' }}}
-       Instr Executable @ E
-       {{{ RET NextIV;
-           PC ↦ᵣ WCap pc_p pc_b pc_e pc_a'
-              ∗ pc_a ↦ₐ w
-              ∗ dst ↦ᵣ WCap p b e a
-              ∗ a ↦ₐ WCap pc_p pc_b pc_e pc_a }}}.
-   Proof.
-     intros. iIntros "(>HPC & >Hpc_a & >Hdst & >Ha) Hφ".
-     destruct (a =? pc_a)%a eqn:Ha.
-     { rewrite (_: a = pc_a); cycle 1.
-       apply Z.eqb_eq in Ha; solve_addr.
-       by iDestruct (addr_dupl_false with "Ha Hpc_a") as "?". }
-     iApply (wp_store_success_reg' with "[$HPC $Hpc_a $Hdst Ha]"); eauto.
-     rewrite Ha. iFrame. iNext. iIntros "(? & ? & ? & ?)". rewrite Ha.
-     iApply "Hφ". iFrame.
-  Qed.
+  (*   iApply (wp_store with "[$Hmap $Hmem]"); eauto; simplify_map_eq; eauto. *)
+  (*   { by rewrite !dom_insert; set_solver+. } *)
+  (*   { eapply mem_eq_implies_allow_store_map; eauto. *)
+  (*     all: by simplify_map_eq. } *)
+  (*   iNext. iIntros (regs' mem' retv) "(#Hspec & Hmem & Hmap)". *)
+  (*   iDestruct "Hspec" as %Hspec. *)
 
-   Lemma wp_store_success_reg_same' E pc_p pc_b pc_e pc_a pc_a' w dst
-         p b e :
-     decodeInstrW w = Store dst (inr dst) →
-     isCorrectPC (WCap pc_p pc_b pc_e pc_a) →
-     (pc_a + 1)%a = Some pc_a' →
-     writeAllowed p = true → withinBounds b e pc_a = true →
+  (*   destruct Hspec.  *)
+  (*    { (* Success *) *)
+  (*      iApply "Hφ". *)
+  (*      destruct H3 as [Hrr2 _]. simplify_map_eq. *)
+  (*      rewrite memMap_resource_1. *)
+  (*      incrementPC_inv. *)
+  (*      simplify_map_eq. *)
+  (*      do 2 rewrite insert_insert. *)
+  (*      iDestruct (regs_of_map_1 with "[$Hmap]") as "HPC"; eauto. iFrame. } *)
+  (*     { (* Failure (contradiction) *) *)
+  (*      destruct X; try incrementPC_inv; simplify_map_eq; eauto. *)
+  (*      apply isCorrectPC_ra_wb in Hvpc. apply andb_prop_elim in Hvpc as [_ Hwb]. *)
+  (*      destruct o; last apply Is_true_false in H2. congruence. done. congruence. *)
+  (*    } *)
+  (*   Qed. *)
 
-     {{{ ▷ PC ↦ᵣ WCap pc_p pc_b pc_e pc_a
-           ∗ ▷ pc_a ↦ₐ w
-           ∗ ▷ dst ↦ᵣ WCap p b e pc_a }}}
-       Instr Executable @ E
-       {{{ RET NextIV;
-           PC ↦ᵣ WCap pc_p pc_b pc_e pc_a'
-              ∗ pc_a ↦ₐ WCap p b e pc_a
-              ∗ dst ↦ᵣ WCap p b e pc_a }}}.
-   Proof.
-     iIntros (Hinstr Hvpc Hpca' Hwa Hwb φ)
-            "(>HPC & >Hi & >Hdst) Hφ".
-     iDestruct (map_of_regs_2 with "HPC Hdst") as "[Hmap %]".
-     iDestruct (memMap_resource_1 with "Hi") as "Hmem".
+  (*  Lemma wp_store_success_same E pc_p pc_b pc_e pc_a pc_a' w dst z w' *)
+  (*        p b e : *)
+  (*    decodeInstrW w = Store dst (inl z) → *)
+  (*    isCorrectPC (WCap pc_p pc_b pc_e pc_a) → *)
+  (*    (pc_a + 1)%a = Some pc_a' → *)
+  (*    writeAllowed p = true → withinBounds b e pc_a = true → *)
 
-    iApply (wp_store _ pc_p with "[$Hmap $Hmem]"); eauto; simplify_map_eq; eauto.
-    { by rewrite !dom_insert; set_solver+. }
-    { eapply mem_eq_implies_allow_store_map; eauto.
-      all: by simplify_map_eq. }
-    iNext. iIntros (regs' mem' retv) "(#Hspec & Hmem & Hmap)".
-    iDestruct "Hspec" as %Hspec.
+  (*    {{{ ▷ PC ↦ᵣ WCap pc_p pc_b pc_e pc_a *)
+  (*          ∗ ▷ pc_a ↦ₐ w *)
+  (*          ∗ ▷ dst ↦ᵣ WCap p b e pc_a }}} *)
+  (*      Instr Executable @ E *)
+  (*      {{{ RET NextIV; *)
+  (*          PC ↦ᵣ WCap pc_p pc_b pc_e pc_a' *)
+  (*             ∗ pc_a ↦ₐ (WInt z) *)
+  (*             ∗ dst ↦ᵣ WCap p b e pc_a }}}. *)
+  (*   Proof. *)
+  (*    iIntros (Hinstr Hvpc Hpca' Hwa Hwb φ) *)
+  (*           "(>HPC & >Hi & >Hdst) Hφ". *)
+  (*    iDestruct (map_of_regs_2 with "HPC Hdst") as "[Hmap %]". *)
+  (*    iDestruct (memMap_resource_1 with "Hi") as "Hmem". *)
 
-    destruct Hspec. 
-     { (* Success *)
-       iApply "Hφ".
-       destruct H4 as [Hrr2 _]. simplify_map_eq.
-       rewrite memMap_resource_1.
-       incrementPC_inv.
-       simplify_map_eq.
-       do 2 rewrite insert_insert.
-       iDestruct (regs_of_map_2 with "[$Hmap]") as "[HPC Hsrc]"; eauto. iFrame. }
-     { (* Failure (contradiction) *)
-       destruct X; try incrementPC_inv; simplify_map_eq; eauto.
-       destruct o. all: try congruence.
-     }
-   Qed.
+  (*   iApply (wp_store _ pc_p with "[$Hmap $Hmem]"); eauto; simplify_map_eq; eauto. *)
+  (*   { by rewrite !dom_insert; set_solver+. } *)
+  (*   { eapply mem_eq_implies_allow_store_map; eauto. *)
+  (*     all: by simplify_map_eq. } *)
+  (*   iNext. iIntros (regs' mem' retv) "(#Hspec & Hmem & Hmap)". *)
+  (*   iDestruct "Hspec" as %Hspec. *)
 
-   Lemma wp_store_success_reg_same_a E pc_p pc_b pc_e pc_a pc_a' w dst src
-         p b e w'' :
-      decodeInstrW w = Store dst (inr src) →
-     isCorrectPC (WCap pc_p pc_b pc_e pc_a) →
-     (pc_a + 1)%a = Some pc_a' →
-     writeAllowed p = true → withinBounds b e pc_a = true →
+  (*   destruct Hspec.  *)
+  (*    { (* Success *) *)
+  (*      iApply "Hφ". *)
+  (*      destruct H4 as [Hrr2 _]. simplify_map_eq. *)
+  (*      rewrite memMap_resource_1. *)
+  (*      incrementPC_inv. *)
+  (*      simplify_map_eq. *)
+  (*      do 2 rewrite insert_insert. *)
+  (*      iDestruct (regs_of_map_2 with "[$Hmap]") as "[HPC Hsrc]"; eauto. iFrame. } *)
+  (*    { (* Failure (contradiction) *) *)
+  (*      destruct X; try incrementPC_inv; simplify_map_eq; eauto. *)
+  (*      destruct o. all: congruence. *)
+  (*    } *)
+  (*    Qed. *)
 
-     {{{ ▷ PC ↦ᵣ WCap pc_p pc_b pc_e pc_a
-           ∗ ▷ pc_a ↦ₐ w
-           ∗ ▷ src ↦ᵣ w''
-           ∗ ▷ dst ↦ᵣ WCap p b e pc_a }}}
-       Instr Executable @ E
-       {{{ RET NextIV;
-           PC ↦ᵣ WCap pc_p pc_b pc_e pc_a'
-              ∗ pc_a ↦ₐ w''
-              ∗ src ↦ᵣ w''
-              ∗ dst ↦ᵣ WCap p b e pc_a}}}.
-   Proof.
-     iIntros (Hinstr Hvpc Hpca' Hwa Hwb φ)
-             "(>HPC & >Hi & >Hsrc & >Hdst) Hφ".
-     iDestruct (map_of_regs_3 with "HPC Hsrc Hdst") as "[Hmap (%&%&%)]".
-     iDestruct (memMap_resource_1 with "Hi") as "Hmem".
+  (*  Lemma wp_store_success_reg' E pc_p pc_b pc_e pc_a pc_a' w dst w' *)
+  (*        p b e a : *)
+  (*     decodeInstrW w = Store dst (inr PC) → *)
+  (*    isCorrectPC (WCap pc_p pc_b pc_e pc_a) → *)
+  (*    (pc_a + 1)%a = Some pc_a' → *)
+  (*    writeAllowed p = true → withinBounds b e a = true → *)
 
-    iApply (wp_store _ pc_p with "[$Hmap $Hmem]"); eauto; simplify_map_eq; eauto.
-    { by rewrite !dom_insert; set_solver+. }
-    { eapply mem_eq_implies_allow_store_map; eauto.
-      all: by simplify_map_eq. }
-    iNext. iIntros (regs' mem' retv) "(#Hspec & Hmem & Hmap)".
-    iDestruct "Hspec" as %Hspec.
+  (*    {{{ ▷ PC ↦ᵣ WCap pc_p pc_b pc_e pc_a *)
+  (*          ∗ ▷ pc_a ↦ₐ w *)
+  (*          ∗ ▷ dst ↦ᵣ WCap p b e a *)
+  (*          ∗ if (a =? pc_a)%a *)
+  (*            then emp *)
+  (*            else ▷ a ↦ₐ w' }}} *)
+  (*      Instr Executable @ E *)
+  (*      {{{ RET NextIV; *)
+  (*          PC ↦ᵣ WCap pc_p pc_b pc_e pc_a' *)
+  (*             ∗ pc_a ↦ₐ (if (a =? pc_a)%a *)
+  (*                        then (WCap pc_p pc_b pc_e pc_a) *)
+  (*                        else w) *)
+  (*             ∗ dst ↦ᵣ WCap p b e a *)
+  (*             ∗ if (a =? pc_a)%a *)
+  (*               then emp *)
+  (*               else a ↦ₐ (WCap pc_p pc_b pc_e pc_a) }}}. *)
+  (*  Proof. *)
+  (*    iIntros (Hinstr Hvpc Hpca' Hwa Hwb φ) *)
+  (*           "(>HPC & >Hi & >Hdst & Ha) Hφ". *)
+  (*    iDestruct (map_of_regs_2 with "HPC Hdst") as "[Hmap %]". *)
+  (*    iDestruct (memMap_resource_2gen_clater _ _ _ _ (λ a w, a ↦ₐ w)%I  with "Hi Ha") as (mem) "[>Hmem %]". *)
 
-    destruct Hspec. 
-     { (* Success *)
-       iApply "Hφ".
-       destruct H6 as [Hrr2 _]. simplify_map_eq.
-       rewrite memMap_resource_1.
-       incrementPC_inv.
-       simplify_map_eq.
-       do 2 rewrite insert_insert.
-       iDestruct (regs_of_map_3 with "[$Hmap]") as "[HPC [Hsrc Hdst] ]"; eauto. iFrame. }
-     { (* Failure (contradiction) *)
-       destruct X; try incrementPC_inv; simplify_map_eq; eauto.
-       destruct o. all: try congruence.
-     }
-   Qed.
+  (*   iApply (wp_store with "[$Hmap $Hmem]"); eauto; simplify_map_eq; eauto. *)
+  (*   { by rewrite !dom_insert; set_solver+. } *)
+  (*   { destruct (a =? pc_a)%a; by simplify_map_eq. } *)
+  (*   { eapply mem_implies_allow_store_map; eauto. all: by simplify_map_eq. } *)
 
-   Lemma wp_store_success_reg E pc_p pc_b pc_e pc_a pc_a' w dst src w'
-         p b e a w'' :
-      decodeInstrW w = Store dst (inr src) →
-     isCorrectPC (WCap pc_p pc_b pc_e pc_a) →
-     (pc_a + 1)%a = Some pc_a' →
-     writeAllowed p = true → withinBounds b e a = true →
+  (*   iNext. iIntros (regs' mem' retv) "(#Hspec & Hmem & Hmap)". *)
+  (*   iDestruct "Hspec" as %Hspec. *)
 
-     {{{ ▷ PC ↦ᵣ WCap pc_p pc_b pc_e pc_a
-           ∗ ▷ pc_a ↦ₐ w
-           ∗ ▷ src ↦ᵣ w''
-           ∗ ▷ dst ↦ᵣ WCap p b e a
-           ∗ ▷ a ↦ₐ w' }}}
-       Instr Executable @ E
-       {{{ RET NextIV;
-           PC ↦ᵣ WCap pc_p pc_b pc_e pc_a'
-              ∗ pc_a ↦ₐ w
-              ∗ src ↦ᵣ w''
-              ∗ dst ↦ᵣ WCap p b e a
-              ∗ a ↦ₐ w'' }}}.
-    Proof.
-      iIntros (Hinstr Hvpc Hpca' Hwa Hwb φ)
-             "(>HPC & >Hi & >Hsrc & >Hdst & >Hsrca) Hφ".
-    iDestruct (map_of_regs_3 with "HPC Hsrc Hdst") as "[Hmap (%&%&%)]".
-    iDestruct (memMap_resource_2ne_apply with "Hi Hsrca") as "[Hmem %]"; auto.
+  (*   destruct Hspec.  *)
+  (*    { (* Success *) *)
+  (*      iApply "Hφ". *)
+  (*      destruct H5 as [Hrr2 _]. simplify_map_eq. *)
+  (*      destruct (a0 =? pc_a)%a eqn:Heq; subst mem. *)
+  (*      -  apply Z.eqb_eq, finz_to_z_eq in Heq. subst a0. *)
+  (*         rewrite insert_insert. *)
+  (*         rewrite memMap_resource_1. *)
+  (*         incrementPC_inv. *)
+  (*         simplify_map_eq. rewrite insert_insert. *)
+  (*         iDestruct (regs_of_map_2 with "[$Hmap]") as "[HPC Hsrc]"; eauto. iFrame. *)
 
-    iApply (wp_store _ pc_p with "[$Hmap $Hmem]"); eauto; simplify_map_eq; eauto.
-    { by rewrite !dom_insert; set_solver+. }
-    { eapply mem_neq_implies_allow_store_map with (a := a); eauto.
-      all: by simplify_map_eq. }
-    iNext. iIntros (regs' mem' retv) "(#Hspec & Hmem & Hmap)".
-    iDestruct "Hspec" as %Hspec.
+  (*      - apply Z.eqb_neq in Heq. *)
+  (*        rewrite insert_commute; last congruence. rewrite insert_insert. *)
+  (*        iDestruct (memMap_resource_2ne with "Hmem") as "[Ha0 Hpc_a]"; first congruence. *)
+  (*        incrementPC_inv. *)
+  (*        rewrite lookup_insert_ne in H6; last congruence. simplify_map_eq. rewrite insert_insert. *)
+  (*        iDestruct (regs_of_map_2 with "[$Hmap]") as "[HPC Hsrc]"; eauto. iFrame. *)
+  (*    } *)
+  (*    { (* Failure (contradiction) *) *)
+  (*      destruct X; try incrementPC_inv; simplify_map_eq; eauto. *)
+  (*      destruct o. all: try congruence. *)
+  (*    } *)
+  (*  Qed. *)
 
-    destruct Hspec. 
-     { (* Success *)
-       iApply "Hφ".
-       destruct H7 as [Hrr2 _]. simplify_map_eq.
-       rewrite insert_commute // insert_insert.
-       iDestruct (memMap_resource_2ne with "Hmem") as "[Hpc_a Ha]";auto.
-       incrementPC_inv.
-       simplify_map_eq.
-       rewrite insert_insert.
-       iDestruct (regs_of_map_3 with "[$Hmap]") as "[HPC [Hsrc Hdst] ]"; eauto. iFrame. }
-     { (* Failure (contradiction) *)
-       destruct X; try incrementPC_inv; simplify_map_eq; eauto.
-       destruct o. all: try congruence.
-     }
-    Qed.
+  (*  Lemma wp_store_success_reg_frominstr_same E pc_p pc_b pc_e pc_a pc_a' w dst w' *)
+  (*        p b e : *)
+  (*     decodeInstrW w = Store dst (inr PC) → *)
+  (*    isCorrectPC (WCap pc_p pc_b pc_e pc_a) → *)
+  (*    (pc_a + 1)%a = Some pc_a' → *)
+  (*    writeAllowed p = true → *)
+  (*    withinBounds b e pc_a = true → *)
 
-   Lemma wp_store_success_reg_same E pc_p pc_b pc_e pc_a pc_a' w dst w'
-         p b e a :
-     decodeInstrW w = Store dst (inr dst) →
-     isCorrectPC (WCap pc_p pc_b pc_e pc_a) →
-     (pc_a + 1)%a = Some pc_a' →
-     writeAllowed p = true → withinBounds b e a = true →
+  (*    {{{ ▷ PC ↦ᵣ WCap pc_p pc_b pc_e pc_a *)
+  (*          ∗ ▷ pc_a ↦ₐ w *)
+  (*          ∗ ▷ dst ↦ᵣ WCap p b e pc_a }}} *)
+  (*      Instr Executable @ E *)
+  (*      {{{ RET NextIV; *)
+  (*          PC ↦ᵣ WCap pc_p pc_b pc_e pc_a' *)
+  (*             ∗ pc_a ↦ₐ WCap pc_p pc_b pc_e pc_a *)
+  (*             ∗ dst ↦ᵣ WCap p b e pc_a }}}. *)
+  (*  Proof. *)
+  (*    intros. iIntros "(HPC & Hpc_a & Hdst) Hφ". *)
+  (*    iApply (wp_store_success_reg' with "[$HPC $Hpc_a $Hdst]"); eauto. *)
+  (*    { rewrite Z.eqb_refl. eauto. } *)
+  (*    iNext. iIntros "(? & ? & ? & ?)". rewrite Z.eqb_refl. *)
+  (*    iApply "Hφ". iFrame. Unshelve. eauto. *)
+  (*  Qed. *)
 
-     {{{ ▷ PC ↦ᵣ WCap pc_p pc_b pc_e pc_a
-           ∗ ▷ pc_a ↦ₐ w
-           ∗ ▷ dst ↦ᵣ WCap p b e a
-           ∗ ▷ a ↦ₐ w' }}}
-       Instr Executable @ E
-       {{{ RET NextIV;
-           PC ↦ᵣ WCap pc_p pc_b pc_e pc_a'
-              ∗ pc_a ↦ₐ w
-              ∗ dst ↦ᵣ WCap p b e a
-              ∗ a ↦ₐ WCap p b e a }}}.
-   Proof.
-    iIntros (Hinstr Hvpc Hpca' Hwa Hwb φ)
-             "(>HPC & >Hi & >Hdst & >Hsrca) Hφ".
-    iDestruct (map_of_regs_2 with "HPC Hdst") as "[Hmap %]".
-    iDestruct (memMap_resource_2ne_apply with "Hi Hsrca") as "[Hmem %]"; auto.
+  (*  Lemma wp_store_success_reg_frominstr E pc_p pc_b pc_e pc_a pc_a' w dst w' *)
+  (*        p b e a : *)
+  (*     decodeInstrW w = Store dst (inr PC) → *)
+  (*    isCorrectPC (WCap pc_p pc_b pc_e pc_a) → *)
+  (*    (pc_a + 1)%a = Some pc_a' → *)
+  (*    writeAllowed p = true → *)
+  (*    withinBounds b e a = true → *)
 
-    iApply (wp_store _ pc_p with "[$Hmap $Hmem]"); eauto; simplify_map_eq; eauto.
-    { by rewrite !dom_insert; set_solver+. }
-    { eapply mem_neq_implies_allow_store_map with (a := a); eauto.
-      all: by simplify_map_eq. }
-    iNext. iIntros (regs' mem' retv) "(#Hspec & Hmem & Hmap)".
-    iDestruct "Hspec" as %Hspec.
+  (*    {{{ ▷ PC ↦ᵣ WCap pc_p pc_b pc_e pc_a *)
+  (*          ∗ ▷ pc_a ↦ₐ w *)
+  (*          ∗ ▷ dst ↦ᵣ WCap p b e a *)
+  (*          ∗ ▷ a ↦ₐ w' }}} *)
+  (*      Instr Executable @ E *)
+  (*      {{{ RET NextIV; *)
+  (*          PC ↦ᵣ WCap pc_p pc_b pc_e pc_a' *)
+  (*             ∗ pc_a ↦ₐ w *)
+  (*             ∗ dst ↦ᵣ WCap p b e a *)
+  (*             ∗ a ↦ₐ WCap pc_p pc_b pc_e pc_a }}}. *)
+  (*  Proof. *)
+  (*    intros. iIntros "(>HPC & >Hpc_a & >Hdst & >Ha) Hφ". *)
+  (*    destruct (a =? pc_a)%a eqn:Ha. *)
+  (*    { rewrite (_: a = pc_a); cycle 1. *)
+  (*      apply Z.eqb_eq in Ha; solve_addr. *)
+  (*      by iDestruct (addr_dupl_false with "Ha Hpc_a") as "?". } *)
+  (*    iApply (wp_store_success_reg' with "[$HPC $Hpc_a $Hdst Ha]"); eauto. *)
+  (*    rewrite Ha. iFrame. iNext. iIntros "(? & ? & ? & ?)". rewrite Ha. *)
+  (*    iApply "Hφ". iFrame. *)
+  (* Qed. *)
 
-    destruct Hspec. 
-     { (* Success *)
-       iApply "Hφ".
-       destruct H5 as [Hrr2 _]. simplify_map_eq.
-       rewrite insert_commute // insert_insert.
-       iDestruct (memMap_resource_2ne with "Hmem") as "[Hpc_a Ha]";auto.
-       incrementPC_inv.
-       simplify_map_eq.
-       rewrite insert_insert.
-       iDestruct (regs_of_map_2 with "[$Hmap]") as "[HPC Hdst]"; eauto. iFrame. }
-     { (* Failure (contradiction) *)
-       destruct X; try incrementPC_inv; simplify_map_eq; eauto.
-       destruct o. all: try congruence.
-     }
-    Qed.
+  (*  Lemma wp_store_success_reg_same' E pc_p pc_b pc_e pc_a pc_a' w dst *)
+  (*        p b e : *)
+  (*    decodeInstrW w = Store dst (inr dst) → *)
+  (*    isCorrectPC (WCap pc_p pc_b pc_e pc_a) → *)
+  (*    (pc_a + 1)%a = Some pc_a' → *)
+  (*    writeAllowed p = true → withinBounds b e pc_a = true → *)
 
-   Lemma wp_store_success_z E pc_p pc_b pc_e pc_a pc_a' w dst z w'
-         p b e a :
-     decodeInstrW w = Store dst (inl z) →
-     isCorrectPC (WCap pc_p pc_b pc_e pc_a) →
-     (pc_a + 1)%a = Some pc_a' →
-     writeAllowed p = true → withinBounds b e a = true →
+  (*    {{{ ▷ PC ↦ᵣ WCap pc_p pc_b pc_e pc_a *)
+  (*          ∗ ▷ pc_a ↦ₐ w *)
+  (*          ∗ ▷ dst ↦ᵣ WCap p b e pc_a }}} *)
+  (*      Instr Executable @ E *)
+  (*      {{{ RET NextIV; *)
+  (*          PC ↦ᵣ WCap pc_p pc_b pc_e pc_a' *)
+  (*             ∗ pc_a ↦ₐ WCap p b e pc_a *)
+  (*             ∗ dst ↦ᵣ WCap p b e pc_a }}}. *)
+  (*  Proof. *)
+  (*    iIntros (Hinstr Hvpc Hpca' Hwa Hwb φ) *)
+  (*           "(>HPC & >Hi & >Hdst) Hφ". *)
+  (*    iDestruct (map_of_regs_2 with "HPC Hdst") as "[Hmap %]". *)
+  (*    iDestruct (memMap_resource_1 with "Hi") as "Hmem". *)
 
-     {{{ ▷ PC ↦ᵣ WCap pc_p pc_b pc_e pc_a
-           ∗ ▷ pc_a ↦ₐ w
-           ∗ ▷ dst ↦ᵣ WCap p b e a
-           ∗ ▷ a ↦ₐ w' }}}
-       Instr Executable @ E
-       {{{ RET NextIV;
-           PC ↦ᵣ WCap pc_p pc_b pc_e pc_a'
-              ∗ pc_a ↦ₐ w
-              ∗ dst ↦ᵣ WCap p b e a
-              ∗ a ↦ₐ WInt z }}}.
-   Proof.
-     iIntros (Hinstr Hvpc Hpca' Hwa Hwb φ)
-             "(>HPC & >Hi & >Hdst & >Hsrca) Hφ".
-    iDestruct (map_of_regs_2 with "HPC Hdst") as "[Hmap %]".
-    iDestruct (memMap_resource_2ne_apply with "Hi Hsrca") as "[Hmem %]"; auto.
+  (*   iApply (wp_store _ pc_p with "[$Hmap $Hmem]"); eauto; simplify_map_eq; eauto. *)
+  (*   { by rewrite !dom_insert; set_solver+. } *)
+  (*   { eapply mem_eq_implies_allow_store_map; eauto. *)
+  (*     all: by simplify_map_eq. } *)
+  (*   iNext. iIntros (regs' mem' retv) "(#Hspec & Hmem & Hmap)". *)
+  (*   iDestruct "Hspec" as %Hspec. *)
 
-    iApply (wp_store _ pc_p with "[$Hmap $Hmem]"); eauto; simplify_map_eq; eauto.
-    { by rewrite !dom_insert; set_solver+. }
-    { eapply mem_neq_implies_allow_store_map with (a := a); eauto.
-      all: by simplify_map_eq. }
-    iNext. iIntros (regs' mem' retv) "(#Hspec & Hmem & Hmap)".
-    iDestruct "Hspec" as %Hspec.
+  (*   destruct Hspec.  *)
+  (*    { (* Success *) *)
+  (*      iApply "Hφ". *)
+  (*      destruct H4 as [Hrr2 _]. simplify_map_eq. *)
+  (*      rewrite memMap_resource_1. *)
+  (*      incrementPC_inv. *)
+  (*      simplify_map_eq. *)
+  (*      do 2 rewrite insert_insert. *)
+  (*      iDestruct (regs_of_map_2 with "[$Hmap]") as "[HPC Hsrc]"; eauto. iFrame. } *)
+  (*    { (* Failure (contradiction) *) *)
+  (*      destruct X; try incrementPC_inv; simplify_map_eq; eauto. *)
+  (*      destruct o. all: try congruence. *)
+  (*    } *)
+  (*  Qed. *)
 
-    destruct Hspec. 
-     { (* Success *)
-       iApply "Hφ".
-       destruct H5 as [Hrr2 _]. simplify_map_eq.
-       rewrite insert_commute // insert_insert.
-       iDestruct (memMap_resource_2ne with "Hmem") as "[Hpc_a Ha]";auto.
-       incrementPC_inv.
-       simplify_map_eq.
-       rewrite insert_insert.
-       iDestruct (regs_of_map_2 with "[$Hmap]") as "[HPC Hdst]"; eauto. iFrame. }
-     { (* Failure (contradiction) *)
-       destruct X; try incrementPC_inv; simplify_map_eq; eauto.
-       destruct o. all: try congruence.
-     }
-    Qed.
+  (*  Lemma wp_store_success_reg_same_a E pc_p pc_b pc_e pc_a pc_a' w dst src *)
+  (*        p b e w'' : *)
+  (*     decodeInstrW w = Store dst (inr src) → *)
+  (*    isCorrectPC (WCap pc_p pc_b pc_e pc_a) → *)
+  (*    (pc_a + 1)%a = Some pc_a' → *)
+  (*    writeAllowed p = true → withinBounds b e pc_a = true → *)
+
+  (*    {{{ ▷ PC ↦ᵣ WCap pc_p pc_b pc_e pc_a *)
+  (*          ∗ ▷ pc_a ↦ₐ w *)
+  (*          ∗ ▷ src ↦ᵣ w'' *)
+  (*          ∗ ▷ dst ↦ᵣ WCap p b e pc_a }}} *)
+  (*      Instr Executable @ E *)
+  (*      {{{ RET NextIV; *)
+  (*          PC ↦ᵣ WCap pc_p pc_b pc_e pc_a' *)
+  (*             ∗ pc_a ↦ₐ w'' *)
+  (*             ∗ src ↦ᵣ w'' *)
+  (*             ∗ dst ↦ᵣ WCap p b e pc_a}}}. *)
+  (*  Proof. *)
+  (*    iIntros (Hinstr Hvpc Hpca' Hwa Hwb φ) *)
+  (*            "(>HPC & >Hi & >Hsrc & >Hdst) Hφ". *)
+  (*    iDestruct (map_of_regs_3 with "HPC Hsrc Hdst") as "[Hmap (%&%&%)]". *)
+  (*    iDestruct (memMap_resource_1 with "Hi") as "Hmem". *)
+
+  (*   iApply (wp_store _ pc_p with "[$Hmap $Hmem]"); eauto; simplify_map_eq; eauto. *)
+  (*   { by rewrite !dom_insert; set_solver+. } *)
+  (*   { eapply mem_eq_implies_allow_store_map; eauto. *)
+  (*     all: by simplify_map_eq. } *)
+  (*   iNext. iIntros (regs' mem' retv) "(#Hspec & Hmem & Hmap)". *)
+  (*   iDestruct "Hspec" as %Hspec. *)
+
+  (*   destruct Hspec.  *)
+  (*    { (* Success *) *)
+  (*      iApply "Hφ". *)
+  (*      destruct H6 as [Hrr2 _]. simplify_map_eq. *)
+  (*      rewrite memMap_resource_1. *)
+  (*      incrementPC_inv. *)
+  (*      simplify_map_eq. *)
+  (*      do 2 rewrite insert_insert. *)
+  (*      iDestruct (regs_of_map_3 with "[$Hmap]") as "[HPC [Hsrc Hdst] ]"; eauto. iFrame. } *)
+  (*    { (* Failure (contradiction) *) *)
+  (*      destruct X; try incrementPC_inv; simplify_map_eq; eauto. *)
+  (*      destruct o. all: try congruence. *)
+  (*    } *)
+  (*  Qed. *)
+
+  (*  Lemma wp_store_success_reg E pc_p pc_b pc_e pc_a pc_a' w dst src w' *)
+  (*        p b e a w'' : *)
+  (*     decodeInstrW w = Store dst (inr src) → *)
+  (*    isCorrectPC (WCap pc_p pc_b pc_e pc_a) → *)
+  (*    (pc_a + 1)%a = Some pc_a' → *)
+  (*    writeAllowed p = true → withinBounds b e a = true → *)
+
+  (*    {{{ ▷ PC ↦ᵣ WCap pc_p pc_b pc_e pc_a *)
+  (*          ∗ ▷ pc_a ↦ₐ w *)
+  (*          ∗ ▷ src ↦ᵣ w'' *)
+  (*          ∗ ▷ dst ↦ᵣ WCap p b e a *)
+  (*          ∗ ▷ a ↦ₐ w' }}} *)
+  (*      Instr Executable @ E *)
+  (*      {{{ RET NextIV; *)
+  (*          PC ↦ᵣ WCap pc_p pc_b pc_e pc_a' *)
+  (*             ∗ pc_a ↦ₐ w *)
+  (*             ∗ src ↦ᵣ w'' *)
+  (*             ∗ dst ↦ᵣ WCap p b e a *)
+  (*             ∗ a ↦ₐ w'' }}}. *)
+  (*   Proof. *)
+  (*     iIntros (Hinstr Hvpc Hpca' Hwa Hwb φ) *)
+  (*            "(>HPC & >Hi & >Hsrc & >Hdst & >Hsrca) Hφ". *)
+  (*   iDestruct (map_of_regs_3 with "HPC Hsrc Hdst") as "[Hmap (%&%&%)]". *)
+  (*   iDestruct (memMap_resource_2ne_apply with "Hi Hsrca") as "[Hmem %]"; auto. *)
+
+  (*   iApply (wp_store _ pc_p with "[$Hmap $Hmem]"); eauto; simplify_map_eq; eauto. *)
+  (*   { by rewrite !dom_insert; set_solver+. } *)
+  (*   { eapply mem_neq_implies_allow_store_map with (a := a); eauto. *)
+  (*     all: by simplify_map_eq. } *)
+  (*   iNext. iIntros (regs' mem' retv) "(#Hspec & Hmem & Hmap)". *)
+  (*   iDestruct "Hspec" as %Hspec. *)
+
+  (*   destruct Hspec.  *)
+  (*    { (* Success *) *)
+  (*      iApply "Hφ". *)
+  (*      destruct H7 as [Hrr2 _]. simplify_map_eq. *)
+  (*      rewrite insert_commute // insert_insert. *)
+  (*      iDestruct (memMap_resource_2ne with "Hmem") as "[Hpc_a Ha]";auto. *)
+  (*      incrementPC_inv. *)
+  (*      simplify_map_eq. *)
+  (*      rewrite insert_insert. *)
+  (*      iDestruct (regs_of_map_3 with "[$Hmap]") as "[HPC [Hsrc Hdst] ]"; eauto. iFrame. } *)
+  (*    { (* Failure (contradiction) *) *)
+  (*      destruct X; try incrementPC_inv; simplify_map_eq; eauto. *)
+  (*      destruct o. all: try congruence. *)
+  (*    } *)
+  (*   Qed. *)
+
+  (*  Lemma wp_store_success_reg_same E pc_p pc_b pc_e pc_a pc_a' w dst w' *)
+  (*        p b e a : *)
+  (*    decodeInstrW w = Store dst (inr dst) → *)
+  (*    isCorrectPC (WCap pc_p pc_b pc_e pc_a) → *)
+  (*    (pc_a + 1)%a = Some pc_a' → *)
+  (*    writeAllowed p = true → withinBounds b e a = true → *)
+
+  (*    {{{ ▷ PC ↦ᵣ WCap pc_p pc_b pc_e pc_a *)
+  (*          ∗ ▷ pc_a ↦ₐ w *)
+  (*          ∗ ▷ dst ↦ᵣ WCap p b e a *)
+  (*          ∗ ▷ a ↦ₐ w' }}} *)
+  (*      Instr Executable @ E *)
+  (*      {{{ RET NextIV; *)
+  (*          PC ↦ᵣ WCap pc_p pc_b pc_e pc_a' *)
+  (*             ∗ pc_a ↦ₐ w *)
+  (*             ∗ dst ↦ᵣ WCap p b e a *)
+  (*             ∗ a ↦ₐ WCap p b e a }}}. *)
+  (*  Proof. *)
+  (*   iIntros (Hinstr Hvpc Hpca' Hwa Hwb φ) *)
+  (*            "(>HPC & >Hi & >Hdst & >Hsrca) Hφ". *)
+  (*   iDestruct (map_of_regs_2 with "HPC Hdst") as "[Hmap %]". *)
+  (*   iDestruct (memMap_resource_2ne_apply with "Hi Hsrca") as "[Hmem %]"; auto. *)
+
+  (*   iApply (wp_store _ pc_p with "[$Hmap $Hmem]"); eauto; simplify_map_eq; eauto. *)
+  (*   { by rewrite !dom_insert; set_solver+. } *)
+  (*   { eapply mem_neq_implies_allow_store_map with (a := a); eauto. *)
+  (*     all: by simplify_map_eq. } *)
+  (*   iNext. iIntros (regs' mem' retv) "(#Hspec & Hmem & Hmap)". *)
+  (*   iDestruct "Hspec" as %Hspec. *)
+
+  (*   destruct Hspec.  *)
+  (*    { (* Success *) *)
+  (*      iApply "Hφ". *)
+  (*      destruct H5 as [Hrr2 _]. simplify_map_eq. *)
+  (*      rewrite insert_commute // insert_insert. *)
+  (*      iDestruct (memMap_resource_2ne with "Hmem") as "[Hpc_a Ha]";auto. *)
+  (*      incrementPC_inv. *)
+  (*      simplify_map_eq. *)
+  (*      rewrite insert_insert. *)
+  (*      iDestruct (regs_of_map_2 with "[$Hmap]") as "[HPC Hdst]"; eauto. iFrame. } *)
+  (*    { (* Failure (contradiction) *) *)
+  (*      destruct X; try incrementPC_inv; simplify_map_eq; eauto. *)
+  (*      destruct o. all: try congruence. *)
+  (*    } *)
+  (*   Qed. *)
+
+  (*  Lemma wp_store_success_z E pc_p pc_b pc_e pc_a pc_a' w dst z w' *)
+  (*        p b e a : *)
+  (*    decodeInstrW w = Store dst (inl z) → *)
+  (*    isCorrectPC (WCap pc_p pc_b pc_e pc_a) → *)
+  (*    (pc_a + 1)%a = Some pc_a' → *)
+  (*    writeAllowed p = true → withinBounds b e a = true → *)
+
+  (*    {{{ ▷ PC ↦ᵣ WCap pc_p pc_b pc_e pc_a *)
+  (*          ∗ ▷ pc_a ↦ₐ w *)
+  (*          ∗ ▷ dst ↦ᵣ WCap p b e a *)
+  (*          ∗ ▷ a ↦ₐ w' }}} *)
+  (*      Instr Executable @ E *)
+  (*      {{{ RET NextIV; *)
+  (*          PC ↦ᵣ WCap pc_p pc_b pc_e pc_a' *)
+  (*             ∗ pc_a ↦ₐ w *)
+  (*             ∗ dst ↦ᵣ WCap p b e a *)
+  (*             ∗ a ↦ₐ WInt z }}}. *)
+  (*  Proof. *)
+  (*    iIntros (Hinstr Hvpc Hpca' Hwa Hwb φ) *)
+  (*            "(>HPC & >Hi & >Hdst & >Hsrca) Hφ". *)
+  (*   iDestruct (map_of_regs_2 with "HPC Hdst") as "[Hmap %]". *)
+  (*   iDestruct (memMap_resource_2ne_apply with "Hi Hsrca") as "[Hmem %]"; auto. *)
+
+  (*   iApply (wp_store _ pc_p with "[$Hmap $Hmem]"); eauto; simplify_map_eq; eauto. *)
+  (*   { by rewrite !dom_insert; set_solver+. } *)
+  (*   { eapply mem_neq_implies_allow_store_map with (a := a); eauto. *)
+  (*     all: by simplify_map_eq. } *)
+  (*   iNext. iIntros (regs' mem' retv) "(#Hspec & Hmem & Hmap)". *)
+  (*   iDestruct "Hspec" as %Hspec. *)
+
+  (*   destruct Hspec.  *)
+  (*    { (* Success *) *)
+  (*      iApply "Hφ". *)
+  (*      destruct H5 as [Hrr2 _]. simplify_map_eq. *)
+  (*      rewrite insert_commute // insert_insert. *)
+  (*      iDestruct (memMap_resource_2ne with "Hmem") as "[Hpc_a Ha]";auto. *)
+  (*      incrementPC_inv. *)
+  (*      simplify_map_eq. *)
+  (*      rewrite insert_insert. *)
+  (*      iDestruct (regs_of_map_2 with "[$Hmap]") as "[HPC Hdst]"; eauto. iFrame. } *)
+  (*    { (* Failure (contradiction) *) *)
+  (*      destruct X; try incrementPC_inv; simplify_map_eq; eauto. *)
+  (*      destruct o. all: try congruence. *)
+  (*    } *)
+  (*   Qed. *)
 
  End cap_lang_rules.
